{
 "cells": [
  {
   "cell_type": "markdown",
   "metadata": {},
   "source": [
    "# Lecture One\n",
    "\n",
    "## Quick Intro???\n",
    "\n",
    "__Theorem__: Assume that $f, g: \\mathbb{R} \\rightarrow \\mathbb{R}$ are continuos on the domain. Let $(A, B) < \\mathbb{R}$, $g(x) \\neq 0 \\forall x \\in (A, B)$. Suppose that $y'(x) = f(x)g(y)$. Then $y(x) = H^{-1}(\\int i(x) dx + c)$...\n",
    "\n",
    "\n",
    "_Example One:_ $y'(t) = r(t)y(t)$. Lets solve this.\n",
    "\n",
    "$$\\begin{align*}\n",
    "&\\frac{dy}{dt} = r(t)y(t),\\\\\n",
    "&\\frac{dy}{y(t)} = r(t)~ dt,\\\\\n",
    "&\\ln|y(t)| = \\int r(t) ~ dt + c, c\\in \\mathbb{R},\\\\\n",
    "&|y(t)| = e^e * ...\\\\\n",
    "\\end{align*}$$\n",
    "\n",
    "_Example Two:_ $y'(t) = \\frac{x}{y}$. Lets solve this.\n",
    "\n",
    "$$\\begin{align*}\n",
    "&\\frac{dy}{dx} = \\frac{x}{y}.\\\\\n",
    "&\\implies y~dy = x~dx \\implies \\int y~ dy - \\int x ~ dx + c\\\\\n",
    "&\\implies \\frac{y^2}{2} = \\frac{x^2}{2} + c \\implies y^2 - x^2 = 2e.\n",
    "\\end{align*}$$\n",
    "\n",
    "Taking a deeper look at the solution $y^2 - x^2 = 2e$, we can solve it as $y = \\pm\\sqrt{x^2 + 2c}$. These are __general explicit solutions__.\n",
    "\n",
    "The equation $y^2 - x^2 = 2e$ is the __general implicit solution__, yes its singular in this case.\n",
    "\n",
    "## 1st Order ODEs, Reducible and Separable\n",
    "\n",
    "What is meant by a reducible equation? Consider the example,\n",
    "\n",
    "_Example Three:_ The Beznoulli equation in the form $y'(x) + a(x)y(x) = b(x)y^{n - 1}(x), n \\in \\mathbb{R}$. Both $a$ and $b$ are continuos functions.\n",
    "\n",
    "We need to find $y(x) = u(x)v(x)$ to help separate the equation.\n",
    "\n",
    "$$\\begin{align*}\n",
    "&y(x) = u(x)v(x) \\implies u'(x)v(x) + u(x)v'(x) + a(x)u(x)v(x) = b(x)(u(x)v(x))^{n - 1},\\\\\n",
    "&u'(x)v(x) + u(x)(v'(x) + a(x)v(x)) = b(x)(u(x)v(x)).\\\\\n",
    "&\\\\\n",
    "&\\text{Find } v(x) : v'(x) + a(x)v(x) = 0.\\\\\n",
    "&v(x) = e^{-\\int a(x)~ dx}.\\\\\n",
    "&\\\\\n",
    "&\\implies u'(x) = b(x)u(x)^{n-1}v(x)^{n-2},\\\\\n",
    "&\\frac{du}{u(x)^{n-1}} = b(x)(v(x))^{n - 2},\\\\\n",
    "&\\implies \\int \\frac{du}{u^{n - 1}} = \\int b(x)(v(x)^{n - 2}) + c.\\\\\n",
    "&\\implies \\int u^{1 - n (?)} = \\begin{cases}&ln|u|\\\\&H(u) (?)\\end{cases}\\\\\n",
    "\\end{align*}$$\n",
    "\n",
    "Equations of the form $y' = f(ax + by + c)$. This is not separable. $a,b,c\\in \\mathbb{R}$ and $f:\\mathbb{R} \\rightarrow \\mathbb{R}$. It however is separable if $a = 0 \\implies y' = f(by + c)$ or $b = 0 \\implies y' = f(ax + c)$. What might be a suitable substitution? Introduce a new function $Z(x) = ax + by(x) + c \\iff y(x) = \\frac{Z(x) - ax - c}{b}$. This is considering the fact that $a, b \\neq 0$. \n",
    "\n",
    "Plug in equations such that $\\frac{Z'(x) - a}{b}$. Another substitution yields $\\frac{Z'(x) - a}{b} = f(Z) \\implies Z'(x) = a + bf(Z)$. This is now a separable ODE.\n",
    "\n",
    "The solution is as follows,\n",
    "\n",
    "$$\\begin{align*}\n",
    "&\\frac{dZ}{a + bf(Z)} = dx \\implies \\int \\frac{dZ}{a + bf(Z)} + c,\\\\\n",
    "&\\\\\n",
    "\\end{align*}$$\n",
    "\n",
    "_Consider the following example:_ $y' = e^{-(3x + y)} - 3$. This is equivalent to $f(t) = e^{-t} - 3$.\n",
    "\n",
    "Solving...\n",
    "\n",
    "$$\\begin{align*}\n",
    "&Z = 3x = y, Z'(x) = 3 + y'(x).\\\\\n",
    "&\\\\\n",
    "&y'(x) = Z'(x) - 3 \\implies Z'(x) - 3 = e^{-Z} - 3.\\\\\n",
    "&Z' = e^{-Z} \\implies \\frac{dZ}{e^{-Z}} = dx,\\\\\n",
    "&e^Z ~dZ = dx \\implies \\int e^Z ~ dZ = x+ c,\\\\\n",
    "&e^Z = x + c, Z = ln(x + c),\\\\\n",
    "&y = ln(x + c) - 3x.\n",
    "\\end{align*}$$\n",
    "\n",
    "## Homogeneous ODEs\n",
    "\n",
    "$y' = f(\\frac{y}{x})$\n",
    "\n",
    "### Homogeneous Functions\n",
    "\n",
    "$f(x, y) = f(\\lambda x, \\lambda y),~ \\forall \\lambda \\neq 0$."
   ]
  }
 ],
 "metadata": {
  "language_info": {
   "name": "python"
  }
 },
 "nbformat": 4,
 "nbformat_minor": 2
}
